interface da classe

Stack.dfy
@@ -8,11 +8,32 @@
 
 class Stack
 {
-  var arr: array<int>
+  var elements: array<nat>;
+  ghost var Elements: array<nat>;
+
+  var top: nat;
+  var size: nat;
   
-  constructor(size: int) requires size >= 0 ensures arr.Length == size 
+  constructor(s: nat) requires s >= 0 
+  ensures size == s
+  ensures top == 0
   {
-    arr := new int[size];
+    size := s;
+    top := 0;
+  }
+
+  predicate Valid() reads this
+  {
+    0 <= size < elements.Length
+  }
+
+  predicate IsEmpty() reads this
+  {
+    top == 0
+  }
+
+  method Size()
+  {
   }
 }
 
